## 1. 
$\lim\limits_{x\rightarrow0}(x^2-\ln^2(1 + x))$

$= \lim\limits_{x\rightarrow0}[x + \ln(1+x)][x - \ln(1 + x)] $

$\sim 2x \cdot \frac{1}{2x^2}$

$= x^3$

## 2.
$\lim\limits_{x\rightarrow0}\frac{e^{\sqrt{1+x^3}} - e^{\sqrt{1-x^3}}}{e}$

$=\frac{e^{\sqrt{1-x^3}}}{e}\cdot(e^{\sqrt{1+x^3}-\sqrt{1-x^3}})$

$\sim \sqrt{1 + x^3} - \sqrt{1-x^3}$

$=\frac{2x^{3}}{\sqrt{1+ x^3}+\sqrt{1-x^3 }} $

$\sim x^3$

## 3.

$\lim\limits_{x \to 0} \frac{\tan x - \sin x}{2x^3} $

$=\frac{1}{2} \lim\limits_{x \to 0} \frac{\tan x}{x} \cdot \frac{1-\cos x}{x^2} $

## 4.
$\lim\limits_{x \to 0} \frac{x^2-\ln^2(1+x)}{x\cos x-x} $
$=\lim\limits_{x\to0}\frac{x+\ln(1+x)}{x}\cdot\frac{x-\ln(1+x)}{\cos x-1}$
